src/m_in/preimage.lean
@@ -1,10 +1,12 @@
-import .basic
+import .minor
 
 open set function 
 
 namespace matroid_in
 
-variables {α β : Type*}
+variables {α β : Type*} 
+
+section preimage
 
 def preimage (M : matroid_in β) [M.finite] (f : α → β) (hf : M.E ⊆ range f) :     
     matroid_in α := 
@@ -50,6 +52,17 @@ def preimage (M : matroid_in β) [M.finite] (f : α → β) (hf : M.E ⊆ range 
       rwa [hB.card_eq_card_of_base hB'.1], 
       end)
     ( fun I hI x hxI, hI.2.subset_ground (mem_image_of_mem _ hxI) )
+
+@[simp] lemma preimage_ground_eq (M : matroid_in β) [M.finite] (f : α → β) (hf : M.E ⊆ range f) : 
+  (M.preimage f hf).E = f ⁻¹' M.E := rfl 
+
+@[simp] lemma preimage_indep_iff (M : matroid_in β) [M.finite] (f : α → β) (hf : M.E ⊆ range f) 
+  (I : set α) : (M.preimage f hf).indep I ↔ inj_on f I ∧ M.indep (f '' I) := by 
+  simp [preimage]
+
+end preimage
+
+section restrict
 
 def restrict' (M : matroid_in α) (X : set α) : matroid_in α :=
 matroid_of_indep X (λ I, M.indep I ∧ I ⊆ X ∩ M.E) ⟨M.empty_indep, empty_subset _⟩ 
@@ -105,12 +118,66 @@ begin
   exact fun h _, h.subset_ground 
 end 
 
+@[simp] lemma restrict'_ground (M : matroid_in α) (X : set α) : (M.restrict' X).E = X := rfl 
+
+end restrict 
+
+section extensions
+
+variables {M : matroid_in α} {e f : α} {I : set α}
+
 def add_loop (M : matroid_in α) (f : α) : matroid_in α := M.restrict' (insert f M.E)
+
+@[simp] lemma add_loop_ground (M : matroid_in α) (f : α) : (M.add_loop f).E = insert f M.E := rfl
+
+@[simp] lemma add_loop_indep_iff : (M.add_loop f).indep I ↔ M.indep I := 
+begin
+  rw [add_loop, restrict'_indep_iff, and_iff_left_iff_imp],
+  exact fun hI, hI.subset_ground.trans (subset_insert _ _), 
+end 
+
+lemma eq_add_loop_iff (M M' : matroid_in α) (hf : f ∉ M.E) : 
+    M' = add_loop M f ↔ M'.loop f ∧ M' ⟍ f = M :=
+begin
+  rw [loop_iff_dep, dep_iff, singleton_subset_iff], 
+  split, 
+  { rintro rfl, 
+    rw [add_loop_indep_iff, add_loop_ground, and_iff_left (mem_insert _ _), indep_singleton, 
+      and_iff_right (show ¬M.nonloop f, from fun h, hf h.mem_ground), 
+      eq_iff_indep_iff_indep_forall, delete_elem, delete_ground, add_loop_ground], 
+    simp only [insert_diff_of_mem, mem_singleton, sdiff_eq_left, disjoint_singleton_right,  
+      delete_indep_iff, add_loop_indep_iff, and_iff_left_iff_imp, and_iff_right hf],
+    rintro I hI - hfI,
+    exact (hI hfI).2 rfl },
+  rintro ⟨hfl,rfl⟩,  
+  apply eq_of_indep_iff_indep_forall _ (fun I hI, _), 
+  { simp only [delete_elem, add_loop_ground, delete_ground, insert_diff_singleton],
+    rw [insert_eq_of_mem hfl.2] },
+  simp only [delete_elem, add_loop_indep_iff, delete_indep_iff, disjoint_singleton_right, 
+    iff_self_and], 
+  exact fun hI' hfI, hfl.1 (hI'.subset (singleton_subset_iff.2 hfI)), 
+end 
 
 def add_coloop (M : matroid_in α) (f : α) : matroid_in α := (M﹡.add_loop f)﹡  
 
+lemma add_coloop_eq (M M' : matroid_in α) (hf : f ∉ M.E) : 
+    M' = add_coloop M f ↔ M'.coloop f ∧ M' ⟍ f = M := 
+begin
+  rw [add_coloop, eq_dual_comm, eq_comm, eq_add_loop_iff _ _ (show f ∉ M﹡.E, from hf), 
+    dual_loop_iff_coloop, eq_dual_comm, delete_elem, dual_delete_dual_eq_contract, 
+    delete_elem, and.congr_right_iff, eq_comm], 
+  intro hf', 
+  rw [contract_eq_delete_of_subset_coloops], 
+  rwa [singleton_subset_iff, ← coloop_iff_mem_cl_empty ], 
+end 
+
+lemma add_coloop_del_eq (M : matroid_in α) (hf : f ∉ M.E) : add_coloop M f ⟍ f = M := 
+  (((M.add_coloop_eq _) hf).1 rfl).2
+
+variable [decidable_eq α] 
+
 /-- extend `e` in `M` by a parallel element `f`. -/
-def parallel_extend [decidable_eq α] (M : matroid_in α) [M.finite] (e f : α) (hf : f ∉ M.E) : 
+def parallel_extend (M : matroid_in α) [M.finite] (e f : α) (hf : f ∉ M.E) : 
     matroid_in α := 
   M.preimage ((@id α).update f e) (begin
     rintro x hx, 
@@ -119,8 +186,180 @@ def parallel_extend [decidable_eq α] (M : matroid_in α) [M.finite] (e f : α) 
     exact hf hx
   end)
 
-def series_extend [decidable_eq α] (M : matroid_in α) [M.finite] (e f : α) (hf : f ∉ M.E) :
+lemma parallel_extend_ground {M : matroid_in α} [M.finite] {e f : α}
+  (he : e ∈ M.E) (hf : f ∉ M.E) : (M.parallel_extend e f hf).E = insert f M.E :=
+begin
+  simp only [matroid_in.preimage_ground_eq, matroid_in.parallel_extend.equations._eqn_1],
+  refine subset_antisymm _ (insert_subset.2 ⟨by simpa, fun x hx, _⟩), 
+  { rintro x hx, 
+    simp only [set.mem_preimage] at hx,
+    obtain (rfl | hx') := eq_or_ne x f, 
+    { exact mem_insert _ _ },
+    rw [update_apply, if_neg hx'] at hx, 
+    exact or.inr hx },
+  obtain (rfl | hx') := eq_or_ne x f,
+  { simpa },
+  rwa [mem_preimage, update_apply, if_neg hx'], 
+end 
+
+lemma image_update_id_apply (x y : α) (s : set α) [decidable (x ∈ s)] : 
+  ((@id α).update x y) '' s = if x ∉ s then s else insert y (s \ {x}) := 
+begin
+  ext a, 
+  simp only [set.mem_image, ite_not], 
+  split_ifs, 
+  { split, 
+    { rintro ⟨x, hx, rfl⟩, 
+      rw [update_apply], 
+      split_ifs, exact mem_insert _ _, 
+      exact or.inr ⟨hx, h_1⟩}, 
+    rintro (rfl | ha), 
+    { refine ⟨_, h, by simp⟩ },  
+    refine ⟨a, ha.1, _⟩, 
+    rw [function.update_noteq, id], 
+    exact fun hax, ha.2 hax },
+  refine ⟨_, fun ha, _⟩, 
+  { rintro ⟨a, ha, rfl⟩,
+    rwa [update_apply, if_neg, id], 
+    exact fun hax, h (hax ▸ ha) },
+  refine ⟨a, ha, _⟩, 
+  rw [update_apply, if_neg, id], 
+  exact fun hax, h (hax ▸ ha)
+end 
+
+lemma pair_subset_iff {x y : α} {s : set α} : {x,y} ⊆ s ↔ x ∈ s ∧ y ∈ s :=
+  by rw [insert_subset, singleton_subset_iff]
+
+lemma eq_parallel_extend (M M' : matroid_in α) [M.finite] {e f : α} (hM' : M'.circuit {e, f}) 
+  (h : M = M' ⟍ f) (hMe : M.nonloop e) (hf : f ∉ M.E) : M' = M.parallel_extend e f hf :=
+begin
+  classical, 
+  have hne : e ≠ f,
+  { rintro rfl, exact hf (hMe.mem_ground), },
+  apply eq_of_indep_iff_indep_forall, 
+  { rw [parallel_extend_ground hMe.mem_ground hf, h, delete_elem, delete_ground, 
+      insert_diff_singleton, eq_comm, insert_eq_self], 
+    exact hM'.subset_ground (by simp) },
+  simp only [parallel_extend, preimage_indep_iff], 
+  refine fun I hIE, ⟨fun hI, ⟨fun x hxI y hyI hxy, _,_⟩, fun hI, _⟩, 
+  { rw [update_apply, update_apply] at hxy, 
+    split_ifs at hxy,
+    { rw [h_1, h_2] },
+    { subst hxy, subst h_1, 
+      refine (hM'.dep.not_indep (hI.subset (show {y,x} ⊆ I, from _))).elim, 
+      rw [insert_subset, singleton_subset_iff],
+      exact ⟨hyI, hxI⟩ },
+    { subst hxy; subst h_2, 
+      refine (hM'.dep.not_indep (hI.subset (show {x,y} ⊆ I, from _))).elim, 
+      rw [insert_subset, singleton_subset_iff],
+      exact ⟨hxI, hyI⟩ },
+    exact hxy },
+  { rw [h, delete_elem, delete_indep_iff, disjoint_singleton_right, mem_image, 
+      image_update_id_apply], 
+    split_ifs, 
+    { have heI : e ∉ I, 
+      { exact fun heI, hM'.dep.not_indep 
+          (hI.subset (insert_subset.2 ⟨heI, singleton_subset_iff.2 h_1⟩)) },
+      refine ⟨_, _⟩, 
+      { rw [indep_iff_forall_subset_not_circuit _], 
+        { rintro C hCss hC, 
+          have hne : C ≠ {e,f}, 
+          { rintro rfl, 
+            rw [pair_comm, insert_diff_singleton_comm ] at hCss, 
+            { exact (hCss (mem_insert _ _)).2 rfl },
+            rintro rfl; exact heI h_1 },
+          obtain ⟨C', hC'ss, hC'⟩ := hC.elimination hM' hne e, 
+          refine hC'.dep.not_indep (hI.subset (hC'ss.trans _)), 
+          rw [diff_subset_iff, union_subset_iff, set.singleton_union, 
+            insert_subset, and_iff_right (mem_insert _ _), singleton_subset_iff], 
+          exact ⟨hCss.trans (insert_subset_insert (diff_subset _ _)), or.inr h_1⟩ },
+        rw [insert_subset],
+        exact ⟨hM'.subset_ground (mem_insert _ _), (diff_subset _ _).trans hIE⟩ },
+      rintro ⟨x, hxI, hx⟩,    
+      obtain (rfl | hxf) := eq_or_ne x f, 
+      { simp only [function.update_same] at hx, subst hx, 
+        exact heI hxI },
+      rw [update_apply, if_neg hxf, id] at hx, 
+      exact hxf hx },
+    rw [and_iff_right hI], 
+    rintro ⟨x, hxI, hx⟩, 
+    have hne : x ≠ f := by rintro rfl; exact h_1 hxI, 
+    rw [update_apply, if_neg hne] at hx, 
+    exact hne hx },
+  rw [image_update_id_apply, h, delete_elem, delete_indep_iff, disjoint_singleton_right] at hI, 
+  split_ifs at hI, swap, 
+  { exact hI.2.1 },
+  rw [indep_iff_forall_subset_not_circuit], 
+  rintro C hCI hC, 
+  
+  have hne : C ≠ {e,f},
+  { rintro rfl, 
+    rw [insert_subset, singleton_subset_iff] at hCI, 
+    refine hne ((hI.1.eq_iff hCI.1 hCI.2).1 _),
+    rw [update_same, update_apply, if_neg hne, id], }, 
+  obtain ⟨C', hC'ss, hC'⟩ := hC.elimination hM' hne f, 
+  refine hC'.dep.not_indep (hI.2.1.subset (hC'ss.trans _)), 
+  simp only [set.diff_singleton_subset_iff, set.union_insert, set.union_singleton],
+  rw [insert_comm f, insert_diff_singleton], 
+  exact insert_subset_insert (insert_subset_insert hCI), 
+end 
+
+lemma parallel_extend_circuit [M.finite] (he : M.nonloop e) (hf : f ∉ M.E) : 
+  (M.parallel_extend e f hf).circuit {e,f} :=
+begin
+  rw [circuit_iff_dep_forall_diff_singleton_indep, dep_iff, 
+    parallel_extend_ground he.mem_ground, parallel_extend, preimage_indep_iff, 
+    image_update_id_apply], 
+  simp only [set.mem_insert_iff, set.mem_singleton, forall_eq_or_imp, not_and,
+    set.insert_diff_of_mem, forall_eq, not_true, if_false, or_true], 
+  have hef : e ≠ f := by rintro rfl; exact hf he.mem_ground,  
+  refine ⟨⟨fun h, _,_⟩, _, _⟩, 
+  { specialize h (mem_insert _ _) (show f ∈ {e,f}, by {rw pair_comm, apply mem_insert}), 
+    rw [update_same, update_apply, if_neg hef, id] at h,
+    exact (hef (h rfl)).elim },
+  { rw [insert_subset, singleton_subset_iff],
+    exact ⟨or.inr he.mem_ground, mem_insert _ _⟩ },
+  { rw [diff_singleton_eq_self (by rwa mem_singleton_iff), preimage_indep_iff, 
+      image_singleton, update_same, indep_singleton, and_iff_left he],
+    apply inj_on_singleton  },
+  rintro _ (rfl : a = f), 
+  rwa [pair_comm, insert_diff_of_mem _ (show a ∈ {a}, by simp), diff_singleton_eq_self, 
+    preimage_indep_iff, and_iff_right (inj_on_singleton _ _), image_singleton, 
+    update_apply, if_neg hef, id, indep_singleton], 
+  rwa [ne_comm] at hef, 
+end 
+
+def series_extend (M : matroid_in α) [M.finite] (e f : α) (hf : f ∉ M.E) :
     matroid_in α := (M﹡.parallel_extend e f hf)﹡ 
+
+lemma eq_series_extend (M M' : matroid_in α) [M.finite] {e f : α} (hM' : M'.cocircuit {e, f}) 
+  (he : e ∈ M.E) (h : M = M' ⟋ f) (hf : f ∉ M.E) (hMe : ¬ M.coloop e) : 
+  M' = M.series_extend e f hf :=
+begin
+  rw [series_extend, eq_dual_comm, eq_comm], 
+  apply eq_parallel_extend, 
+  { rwa [dual_circuit_iff_cocircuit] },
+  { rw [h, contract_elem, contract_dual_eq_dual_delete, delete_elem] },
+  rwa [← dual_loop_iff_coloop, not_loop_iff (show e ∈ M﹡.E, from he)] at hMe,
+end 
+
+lemma cocircuit_contr_elem_eq_series_extend (M : matroid_in α) [M.finite] {e f : α} 
+  (hM : M.cocircuit {e, f}) (he : e ∈ (M ⟋ f).E) (hf : f ∉ (M ⟋ f).E) (hMe : ¬ (M ⟋ f).coloop e) : 
+  series_extend (M ⟋ f) e f hf = M :=
+by { rw [eq_comm], exact eq_series_extend _ _  hM he rfl _ hMe }
+
+-- lemma series_extend_cocircuit (M : matroid_in α) [M.finite] {e f : α} (he : e ∈ M.E) 
+--   (hMe : ¬ M.coloop e) (hf : f ∉ M.E) : (series_extend M e f hf).cocircuit {e, f} := 
+-- begin
+  
+-- end 
+
+-- lemma series_extend_contr_eq (M : matroid_in α) {e f : α} (he : e ∈ M.E) (hf : f ∉ M.E) 
+--   (hMe : ¬ M.coloop e) : M = (series_extend M he hf hMe) ⟋ f := sorry
+
+
+
+end extensions
 
 end matroid_in 
     
